\begin{align*}
& Fibonacci Array \\
& \\
& \sum_{i=0}^nf(i)=f(n+2)-1 \\
& \sum_{i=1}^nf(2i-1)=f(2n) \\
& \sum_{i=1}^nf(2i)=f(2n+1)-1 \\
& \sum_{i=1}^nf^2(i)=f(n)f(n+1) \\
& \sum_{i=1}^nif(i)=nf(n+2)-f(n+3)+2 \\
& f(n-k)f(n+k)-(-1)^{k-n}f^2(n)=f^k(n) \\
& 3f(n)=f(n-2)+f(n+2) \\
& f(m+n-1)=f(m-1)f(n-1)+f(m)f(n) \\
& f(2n-2m-2)(f(2n)+f(2n+2))=f(2m+2)+f(4n-2m) \\
& f(2n-1)=f^2(n)-f^2(n-2) \\
& f(n)=\binom{n-1}{0}+\binom{n-2}{1}+L+\binom{n-1-m}{m} \\
& Lucas Array \\
\end{align*}
$$ L(n)=\left\{
\begin{aligned}
2 & , & x = 1 \\
1 & , & x = 2 \\
L_{n-1}+L_{n-2} & , & x \geq 2
\end{aligned}
\right.
$$
\begin{align*}
& \\
& F_{2n}=F_nL_n \\
& 5F_n=L{n-1}+L{n+1} \\
& L^2_n=5F_n^2+4(-1)^n \\
& \lim\limits_{x \to \infty} \frac{L_n}{F_n} = \sqrt 5 \\
& L_n=F_{n-1}+F_{n+1} \\
& \sum\limits_{k=0}^{n}\binom n k (-1)^kF(k)=-F(n) \\
& \sum\limits_{k=0}^{n}\binom n k (-1)^kL(k)=L(n) \\
& \sum\limits_{k=0}^{n}\binom n k F(k)=F(2n) \\
& \sum\limits_{k=0}^{\lfloor\frac n 2\rfloor}\binom{n-k}{k}=F(n+1) \\
& \sum\limits_{k=0}^{n}\binom k n[f(k)+(-1)^{n-k}\sum\limits_{s=0}^k\binom k sf(s)]F(n-k)=0 \\
& \sum\limits_{k=0}^{n}\binom k n[f(k)-(-1)^{n-k}\sum\limits_{s=0}^k\binom k sf(s)]L(n-k)=0 \\
& \\
& gcd(F(n),F(m))=gcd(n,m) \\
& F(m)|F(n) \leftrightarrow m|n \\
& assert\;p\;is\;prime \\
& F(p-p\left(\frac p 5 \right))\equiv0(mod\;p) \\
& F(p+p\left(\frac p 5 \right))\equiv1(mod\;p) \\
& F(p)\equiv \left(\frac p 5\right)(mod\;p)
\end{align*}

